src/Bedrock/Field/Synthesis/Examples/pallas_prime_certif.v
@@ -2,9 +2,9 @@
    Exports pallas_modulus and prime_pallas.
    Certificate from coqprime/gencertif/prime28948...630337.v *)
 
-Require Import Coq.ZArith.ZArith.
-Require Import Coq.ZArith.Znumtheory.
-Require Import Coq.Lists.List. Import ListNotations.
+From Stdlib Require Import ZArith.ZArith.
+From Stdlib Require Import ZArith.Znumtheory.
+From Stdlib Require Import Lists.List. Import ListNotations.
 From Coqprime Require Import PocklingtonRefl BasePrimes.
 
 Local Open Scope positive_scope.
@@ -30,5 +30,5 @@ Proof.
           (Proof_certif 3 prime3) ::
           (Proof_certif 2 prime2) ::
            nil)).
-  native_cast_no_check (refl_equal true).
+  vm_cast_no_check (refl_equal true).
 Qed.
